WIP: fixing invariant for local

theories/sim/cmra.v
@@ -25,25 +25,20 @@ Definition cmapUR := gmapUR call_id callStateR.
 
 Definition to_cmapUR (cm: cmap) : cmapUR := fmap to_callStateR cm.
 
-Definition tmap := gmap ptr_id (tag_kind * mem).
-Definition heaplet := gmap loc scalar.
+Notation heaplet := mem.
+Definition tmap := gmap ptr_id (tag_kind * heaplet).
 Definition heapletR := gmapR loc (agreeR scalarC).
 (* ptr_id ⇀ TagKid x (loc ⇀ Ag(Scalar)) *)
 Definition tmapUR := gmapUR ptr_id (prodR tagKindR heapletR).
 
-Definition to_heapletR (h: mem) : heapletR := fmap to_agree h.
+Definition to_heapR (h: heaplet) : heapletR := fmap to_agree h.
 Definition to_tmapUR (pm: tmap) : tmapUR :=
-  fmap (λ tm, (to_tagKindR tm.1, to_heapletR tm.2)) pm.
+  fmap (λ tm, (to_tagKindR tm.1, to_heapR tm.2)) pm.
 
-Inductive loc_state := lsLocal (s: scalar) (t: ptr_id) | lsShared.
-Definition loc_stateR := (csumR (exclR (leibnizO (scalar * nat))) unitR).
-Definition lmap := gmap loc (scalar * ptr_id).
-Definition lmapUR := gmapUR loc loc_stateR.
-Definition to_locStateR (ls: loc_state) : loc_stateR :=
-  match ls with
-  | lsLocal s t => Cinl (Excl (s, t))
-  | lsShared => Cinr ()
-  end.
+Definition lmap := gmap loc ptr_id.
+Definition tagR := exclR (leibnizO ptr_id).
+Definition lmapUR := gmapUR loc tagR.
+Definition to_tagR (t: ptr_id) := Excl t.
 
 Definition res := (tmap * cmap * lmap)%type.
 Definition resUR := prodUR (prodUR tmapUR cmapUR) lmapUR.
@@ -270,16 +265,16 @@ Proof.
 Qed.
 
 (** heaplet *)
-Lemma to_heapletR_valid h : ✓ (to_heapletR h).
+Lemma to_heapR_valid h : ✓ (to_heapR h).
 Proof.
-  intros l. rewrite /to_heapletR lookup_fmap.
+  intros l. rewrite /to_heapR lookup_fmap.
   destruct (h !! l) eqn:Eq; rewrite Eq //.
 Qed.
 
-Lemma to_heapletR_lookup h l s :
-  to_heapletR h !! l ≡ Some (to_agree s) → h !! l = Some s.
+Lemma to_heapR_lookup h l s :
+  to_heapR h !! l ≡ Some (to_agree s) → h !! l = Some s.
 Proof.
-  rewrite /to_heapletR lookup_fmap.
+  rewrite /to_heapR lookup_fmap.
   destruct (h !! l) as [s'|] eqn:Eqs; rewrite Eqs /=; [|by inversion 1].
   intros Eq%Some_equiv_inj%to_agree_inj. by inversion Eq.
 Qed.
@@ -298,7 +293,7 @@ Proof.
   intros Eq. move : (VALID l). rewrite lookup_op Eq.
   destruct (lm1 !! l) as [ls2|] eqn:Eql; rewrite Eql; [|by rewrite left_id].
   rewrite -Some_op.
-  destruct ls as [|[]|], ls2 as [|[]|]; simpl; try inversion 1. done.
+  destruct ls, ls2; simpl; try inversion 1.
 Qed.
 
 Lemma lmap_lookup_op_l (lm1 lm2 : lmapUR) (VALID: ✓ (lm1 ⋅ lm2)) l ls :
@@ -307,34 +302,33 @@ Proof.
   intros Eq. move : (VALID l). rewrite lookup_op Eq.
   destruct (lm2 !! l) as [ls2|] eqn:Eql; rewrite Eql; [|by rewrite right_id].
   rewrite -Some_op.
-  destruct ls as [|[]|], ls2 as [|[]|]; simpl; try inversion 1. done.
+  destruct ls, ls2; simpl; try inversion 1.
 Qed.
 
-Lemma lmap_exclusive s stk mb :
-  mb ⋅ Some (to_locStateR (lsLocal s stk)) ≡ Some (to_locStateR lsShared) → False.
+Lemma lmap_lookup_op_included (lm1 lm2 : lmapUR) (l: loc) (t: ptr_id)
+  (VALID: ✓ lm2) (INCL: (lm1 : lmapUR) ≼ (lm2 : lmapUR)):
+  (lm1 !! l : optionR tagR) ≡ Some $ to_tagR t → (lm2 !! l : optionR tagR) ≡ Some $ to_tagR t.
 Proof.
-  destruct mb as [c|]; [rewrite -Some_op|rewrite left_id];
-    intros Eq%Some_equiv_inj.
-  - destruct c as [[]| |]; inversion Eq.
-  - inversion Eq.
+  destruct INCL as [cm' Eq]. rewrite Eq. apply lmap_lookup_op_l. by rewrite -Eq.
 Qed.
 
-Lemma lmap_exclusive_r s stk mb :
-  mb ⋅ Some (to_locStateR lsShared) ≡ Some (to_locStateR (lsLocal s stk)) → False.
-Proof.
-  destruct mb as [c|]; [rewrite -Some_op|rewrite left_id];
-    intros Eq%Some_equiv_inj.
-  - destruct c as [[]| |]; inversion Eq.
-  - inversion Eq.
-Qed.
-
-Lemma lmap_exclusive_2 s1 stk1 s2 stk2 c :
-  Some c ⋅ Some (to_locStateR (lsLocal s1 stk1))
-    ≡ Some (to_locStateR (lsLocal s2 stk2))
-  → False.
+Lemma lmap_exclusive_2 t1 t2 (c: tagR) :
+  Some c ⋅ Some (to_tagR t1) ≡ Some (to_tagR t2) → False.
 Proof.
   rewrite -Some_op. intros Eq%Some_equiv_inj.
-  destruct c as [[]| |]; inversion Eq; simplify_eq.
+  destruct c; inversion Eq.
+Qed.
+
+Lemma tagR_valid (ls: tagR) : valid ls → ∃ t, ls = to_tagR t.
+Proof. destruct ls as [t|]; simpl; [|done]. naive_solver. Qed.
+
+Lemma lmap_exclusive_eq_l t (c: tagR) (mb: optionR tagR) :
+  Some c ⋅ mb ≡ Some (to_tagR t) → c ≡ to_tagR t.
+Proof.
+  intros Eq.
+  have VALID: valid (Some c ⋅ mb) by rewrite Eq. move :Eq.
+  destruct c, mb as [[]|]; simplify_eq; try done.
+  rewrite right_id. by intros ?%Some_equiv_inj.
 Qed.
 
 (** The Core *)
@@ -359,18 +353,17 @@ Definition res_tag tg tk (h: heaplet) : resUR :=
 Definition res_callState (c: call_id) (cs: call_state) : resUR :=
   (ε, {[c := to_callStateR cs]}, ε).
 
-Fixpoint init_local (l:loc) (n:nat) (s: scalar) (t: ptr_id)
-  (ls: gmap loc (scalar * ptr_id)) : gmap loc (scalar * ptr_id) :=
+
+Fixpoint write_local (l:loc) (n:nat) (t: ptr_id) (ls: lmap) : lmap :=
   match n with
   | O => ls
-  | S n => <[l := (s, t)]>(init_local (l +ₗ 1) n s t ls)
+  | S n => <[l := t]>(write_local (l +ₗ 1) n t ls)
   end.
 
-Definition init_local_res l n s t ls : lmapUR :=
-  fmap (λ sstk, to_locStateR $ lsLocal sstk.1 sstk.2) (init_local l n s t ls).
+Definition res_loc l n t : resUR := (ε, fmap to_tagR (write_local l n t ∅)).
 
-Definition res_mapsto (l:loc) (n:nat) (s: scalar) (t: ptr_id) : resUR :=
-  (ε, ε, init_local_res l n s t ∅).
+Definition res_mapsto (l:loc) (v: value) (t: ptr_id) : resUR :=
+  res_loc l (length v) t ⋅ res_tag t tkUnique (write_mem l v ∅).
 
 (** res_tag *)
 Lemma res_tag_alloc_local_update lsf t k h (FRESH: lsf.(rtm) !! t = None) :
@@ -380,15 +373,15 @@ Proof.
   apply prod_local_update_1, prod_local_update_1.
   rewrite cmra_comm -insert_singleton_op //.
   apply alloc_singleton_local_update; [done|].
-  split. by destruct k. apply to_heapletR_valid.
+  split. by destruct k. apply to_heapR_valid.
 Qed.
 
 (** res_mapsto *)
-Lemma init_local_lookup l n s t ls :
+Lemma write_local_lookup l n t ls :
   (∀ (i: nat), (i < n)%nat →
-    init_local l n s t ls !! (l +ₗ i) = Some (s,t)) ∧
+    write_local l n t ls !! (l +ₗ i) = Some t) ∧
   (∀ (l': loc), (∀ (i: nat), (i < n)%nat → l' ≠ l +ₗ i) →
-    init_local l n s t ls !! l' = ls !! l').
+    write_local l n t ls !! l' = ls !! l').
 Proof.
   revert l ls. induction n as [|n IH]; intros l ls; simpl.
   { split; intros ??; [lia|done]. }
@@ -410,13 +403,13 @@ Proof.
     + specialize (Lt O ltac:(lia)). by rewrite shift_loc_0_nat in Lt.
 Qed.
 
-Lemma init_local_lookup_case l n s t ls :
-  ∀ l' s', init_local l n s t ls !! l' = Some s' →
-  ls !! l' = Some s' ∧ (∀ i : nat, (i < n)%nat → l' ≠ l +ₗ i) ∨
+Lemma write_local_lookup_case l n t ls :
+  ∀ l' t', write_local l n t ls !! l' = Some t' →
+  ls !! l' = Some t' ∧ (∀ i : nat, (i < n)%nat → l' ≠ l +ₗ i) ∨
   ∃ i, (0 ≤ i < n) ∧ l' = l +ₗ i.
 Proof.
-  destruct (init_local_lookup l n s t ls) as [EQ1 EQ2].
-  intros l1 s1 Eq'.
+  destruct (write_local_lookup l n t ls) as [EQ1 EQ2].
+  intros l1 t1s1 Eq'.
   case (decide (l1.1 = l.1)) => [Eql|NEql];
     [case (decide (l.2 ≤ l1.2 < l.2 + n)) => [[Le Lt]|NIN]|].
   - have Eql2: l1 = l +ₗ Z.of_nat (Z.to_nat (l1.2 - l.2)). {
@@ -434,121 +427,118 @@ Proof.
     rewrite EQ2 // in Eq'.
 Qed.
 
-Lemma res_mapsto_lookup l n s t :
-  (∀ (i: nat), (i < n)%nat →
-    rlm (res_mapsto l n s t) !! (l +ₗ i) = Some $ to_locStateR $ lsLocal s t) ∧
-  (∀ (l': loc), (∀ (i: nat), (i < n)%nat → l' ≠ l +ₗ i) →
-    rlm (res_mapsto l n s t) !! l' = None).
+Lemma res_mapsto_llookup l v t :
+  (∀ (i: nat), (i < length v)%nat →
+    (res_mapsto l v t).(rlm) !! (l +ₗ i) = Some $ to_tagR t) ∧
+  (∀ (l': loc), (∀ (i: nat), (i < length v)%nat → l' ≠ l +ₗ i) →
+    (res_mapsto l v t).(rlm) !! l' = None).
 Proof.
-  destruct (init_local_lookup l n s t ∅) as [EQ1 EQ2]. split.
-  - intros i Lti. by rewrite /= lookup_fmap (EQ1 _ Lti).
-  - intros l' NEQ. by rewrite /= lookup_fmap (EQ2 _ NEQ).
+  destruct (write_local_lookup l (length v) t ∅) as [EQ1 EQ2]. split.
+  - intros i Lti. by rewrite /= right_id lookup_fmap (EQ1 _ Lti).
+  - intros l' NEQ. by rewrite /= right_id lookup_fmap (EQ2 _ NEQ).
 Qed.
 
-Lemma res_mapsto_lookup_case l n s t :
-  ∀ l' s', rlm (res_mapsto l n s t) !! l' ≡ Some s' →
-  s' = to_locStateR $ lsLocal s t ∧ ∃ i, (0 ≤ i < n) ∧ l' = l +ₗ i.
+Lemma res_mapsto_llookup_case l v t :
+  ∀ l' t', ((res_mapsto l v t).(rlm) !! l' : optionR tagR) ≡ Some t' →
+  t' = to_tagR t ∧ ∃ i, (0 ≤ i < length v) ∧ l' = l +ₗ i.
 Proof.
-  intros l' s' Eq'. apply leibniz_equiv_iff in Eq'.
-  move : Eq'. rewrite /= lookup_fmap.
-  destruct (init_local l n s t ∅ !! l') as [[s1 stk1]|] eqn:Eql'; [|done].
+  intros l' t' Eq'. apply leibniz_equiv_iff in Eq'.
+  move : Eq'. rewrite /= right_id lookup_fmap.
+  destruct (write_local l (length v) t ∅ !! l')
+    as [t1|] eqn:Eql'; rewrite Eql'; [|done].
   simpl. intros. simplify_eq.
-  destruct (init_local_lookup_case _ _ _ _ _ _ _ Eql') as [[]|Eq']; [done|].
+  destruct (write_local_lookup_case _ _ _ _ _ _ Eql') as [[]|Eq']; [done|].
   destruct Eq' as [i [[? Lti] Eqi]].
-  have Lti': (Z.to_nat i < n)%nat by rewrite Nat2Z.inj_lt Z2Nat.id.
-  destruct (init_local_lookup l n s t ∅) as [EQ _].
+  have Lti': (Z.to_nat i < length v)%nat by rewrite Nat2Z.inj_lt Z2Nat.id.
+  destruct (write_local_lookup l (length v) t ∅) as [EQ _].
   specialize (EQ _ Lti'). rewrite Z2Nat.id // -Eqi Eql' in EQ. simplify_eq.
   naive_solver.
 Qed.
 
-Lemma res_mapsto_lookup_shared l n s t lm:
-  ∀ l', rlm (lm ⋅ res_mapsto l n s t) !! l' ≡ Some (to_locStateR lsShared) →
-  rlm lm !! l' ≡  Some (to_locStateR lsShared) ∧
-  (∀ (i: nat), (i < n)%nat → l' ≠ l +ₗ i).
-Proof.
-  intros l'. rewrite lookup_op.
-  destruct (rlm (res_mapsto l n s t) !! l') as [s'|] eqn: Eqs'; rewrite Eqs'.
-  - apply leibniz_equiv_iff, res_mapsto_lookup_case in Eqs' as [Eqs' ?].
-    subst s'. by intros ?%lmap_exclusive.
-  - rewrite right_id. intros. split; [done|].
-    intros i Lt Eq. subst l'.
-    move : Eqs'. rewrite /= lookup_fmap.
-    destruct (init_local_lookup l n s t ∅) as [EQ1 _].
-    by rewrite (EQ1 _ Lt).
-Qed.
+Lemma res_mapsto_tlookup l v (t: ptr_id) :
+  (res_mapsto l v t).(rtm) !! t ≡
+    Some (to_tagKindR tkUnique, to_agree <$> (write_mem l v ∅)).
+Proof. by rewrite lookup_op /= lookup_empty left_id lookup_insert. Qed.
 
-Lemma init_local_plus1 l n s t :
-  init_local (l +ₗ 1) n s t ∅ !! l = None.
+Lemma res_mapsto_tlookup_ne l v (t t': ptr_id) (NEQ: t' ≠ t) :
+  (res_mapsto l v t).(rtm) !! t' ≡ None.
+Proof. by rewrite lookup_op /= lookup_empty left_id lookup_insert_ne. Qed.
+
+Lemma write_local_plus1 l n t :
+  write_local (l +ₗ 1) n t ∅ !! l = None.
 Proof.
-  destruct (init_local_lookup (l +ₗ 1) n s t ∅) as [_ EQ].
+  destruct (write_local_lookup (l +ₗ 1) n t ∅) as [_ EQ].
   rewrite EQ //. intros ??. rewrite shift_loc_assoc -{1}(shift_loc_0 l).
   intros ?%shift_loc_inj. lia.
 Qed.
 
-Lemma init_local_res_S l n s t :
-  init_local_res l (S n) s t ∅ ≡
-  {[l := to_locStateR $ lsLocal s t ]} ⋅ (init_local_res (l +ₗ 1) n s t ∅).
+Lemma write_local_res_S l n t :
+  (to_tagR <$> write_local l (S n) t ∅ : lmapUR) ≡
+  ({[l := to_tagR t]} ⋅ (to_tagR <$> write_local (l +ₗ 1) n t ∅) : lmapUR).
 Proof.
-  rewrite {1}/init_local_res /= fmap_insert /= insert_singleton_op // lookup_fmap.
-  rewrite init_local_plus1 //.
+  rewrite /= fmap_insert /= insert_singleton_op //.
+  rewrite lookup_fmap write_local_plus1 //.
 Qed.
 
-Lemma init_local_res_mem_dom l n s t :
-  dom (gset loc) (init_local_res l n s t ∅) ≡ dom (gset loc) (init_mem l n ∅).
+Lemma write_local_mem_dom l n t :
+  dom (gset loc) (write_local l n t ∅) ≡ dom (gset loc) (init_mem l n ∅).
 Proof.
-  revert l. induction n as [|n IH]; simpl; intros l; rewrite /init_local_res.
-  - by rewrite fmap_empty.
-  - rewrite /= fmap_insert 2!dom_insert IH //.
+  revert l. induction n as [|n IH]; simpl; intros l; [done|].
+  rewrite /= 2!dom_insert IH //.
 Qed.
 
-Lemma init_local_res_local_update lsf l n s t:
+Lemma write_local_res_local_update lsf l n t:
   (∀ i, (i < n)%nat → lsf !! (l +ₗ i) = None) →
-  (lsf, ε) ~l~> (lsf ⋅ init_local_res l n s t ∅, init_local_res l n s t ∅).
+  (lsf, ε) ~l~>
+  (lsf ⋅ (to_tagR <$> write_local l n t ∅) : lmapUR, to_tagR <$> write_local l n t ∅ : lmapUR).
 Proof.
   revert l lsf.
   induction n as [|n IH]; intros l lsf HL.
-  - rewrite /init_local_res /= fmap_empty right_id //.
-  - rewrite /= init_local_res_S.
-    rewrite (cmra_comm {[l := to_locStateR (lsLocal s t)]}
-                       (init_local_res _ _ _ _ _)).
+  - rewrite /= fmap_empty right_id //.
+  - rewrite /= write_local_res_S.
+    rewrite (cmra_comm ({[l := to_tagR t]} : lmapUR) (to_tagR <$> write_local _ _ _ _)).
     rewrite cmra_assoc.
     etrans.
     + apply (IH (l +ₗ 1)).
       intros i Lt. rewrite shift_loc_assoc -(Nat2Z.inj_add 1).
       apply HL. lia.
-    + have NEQ1: init_local_res (l +ₗ 1) n s t ∅ !! l = None.
-      { rewrite {1}/init_local_res lookup_fmap init_local_plus1 //. }
-      have ?: (lsf ⋅ init_local_res (l +ₗ 1) n s t ∅) !! l = None.
-      { rewrite lookup_op NEQ1 right_id_L.
+    + have NEQ1: write_local (l +ₗ 1) n t ∅ !! l = None.
+      { rewrite {1}/write_local write_local_plus1 //. }
+      have ?: (lsf ⋅ (to_tagR <$> write_local (l +ₗ 1) n t ∅)) !! l = None.
+      { rewrite lookup_op lookup_fmap NEQ1 right_id_L.
         specialize (HL O). rewrite shift_loc_0_nat in HL. apply HL. lia. }
-      rewrite 2!(cmra_comm _  {[l := to_locStateR (lsLocal s t)]})
-              -insert_singleton_op // -insert_singleton_op //.
+      rewrite 2!(cmra_comm _  {[l := _]})
+              -insert_singleton_op // -insert_singleton_op;
+        [|by rewrite lookup_fmap NEQ1].
       by apply alloc_local_update.
 Qed.
 
-Lemma res_mapsto_local_alloc_local_update lsf l n s t:
-  (∀ i, (i < n)%nat → lsf.(rlm) !! (l +ₗ i) = None) →
-  (lsf, ε) ~l~> (lsf ⋅ res_mapsto l n s t, res_mapsto l n s t).
+
+Lemma res_mapsto_local_alloc_local_update lsf l v t:
+  lsf.(rtm) !! t = None →
+  (∀ i, (i < length v)%nat → lsf.(rlm) !! (l +ₗ i) = None) →
+  (lsf, ε) ~l~> (lsf ⋅ res_mapsto l v t, res_mapsto l v t).
 Proof.
-  intros. destruct lsf as [[tm cm] lm]. rewrite 2!pair_op 2!right_id.
-  apply prod_local_update_2.
-  by apply init_local_res_local_update.
+  intros FRESH1 FRESH2. destruct lsf as [[tm cm] lm].
+  rewrite /res_mapsto (cmra_comm (res_loc _ _ _)).
+  etrans. by apply (res_tag_alloc_local_update _ t tkUnique (write_mem l v ∅)).
+  rewrite !pair_op !right_id left_id /=. apply prod_local_update_2.
+  by apply write_local_res_local_update.
 Qed.
 
-Lemma res_mapsto_1_insert_local_update (r: resUR) (l: loc) v1 v2 (t: ptr_id)
-  (NONE: r.(rlm) !! l = None):
-  (r ⋅ res_mapsto l 1 v1 t, res_mapsto l 1 v1 t) ~l~>
-  (r ⋅ res_mapsto l 1 v2 t, res_mapsto l 1 v2 t).
+Lemma res_mapsto_1_insert_local_update (r: resUR) (l: loc) s1 s2 (t: ptr_id)
+  (NONE1: r.(rlm) !! l = None) (NONE2: r.(rtm) !! t = None):
+  (r ⋅ res_mapsto l [s1] t, res_mapsto l [s1] t) ~l~>
+  (r ⋅ res_mapsto l [s2] t, res_mapsto l [s2] t).
 Proof.
-  intros. destruct r as [[tm cm] lm]. rewrite 4!pair_op 2!right_id.
-  apply prod_local_update_2.
-  rewrite cmra_comm (cmra_comm _ (init_local_res l 1 v2 t ∅)).
-  rewrite /= /init_local_res /= 2!fmap_insert /= fmap_empty.
-  do 2 rewrite -insert_singleton_op //.
-  rewrite -(insert_insert lm l (to_locStateR $ lsLocal v2 t) (to_locStateR $ lsLocal v1 t)).
-  eapply (singleton_local_update (<[l:=Cinl (Excl (v1, t))]> lm : lmapUR)).
-  { by rewrite lookup_insert. }
-  (* FIXME(Coq bug 6294) : we shouldn't need to assert here. *)
-  assert (Exclusive (A:=loc_stateR) (Cinl (Excl (v1, t)))) by exact: Cinl_exclusive.
-  by apply : exclusive_local_update.
+  intros. destruct r as [[tm cm] lm].
+  rewrite !pair_op !right_id /= !left_id /=.
+  do 2 (rewrite (cmra_comm tm) -insert_singleton_op; [|done]). etrans.
+  - apply prod_local_update_1, prod_local_update_1.
+    rewrite /= left_id.
+    instantiate (1:= {[t := (Cinl (Excl ()), to_agree <$> <[l:=s2]> ∅)]}).
+    eapply (singleton_local_update (<[t := _]> tm : tmapUR)). by rewrite lookup_insert.
+    apply exclusive_local_update. split; [done|apply to_heapR_valid].
+  - rewrite /res_mapsto !right_id_L /= insert_insert /=.
+    rewrite /res_loc /res_tag /= pair_op left_id right_id //.
 Qed.
